Replicated version of one-shot leader election

ReplicatedLeader.fst
@@ -1,4 +1,4 @@
-module ReplicatedOneShot
+module ReplicatedLeader
 
 module M = FStar.Map
 
@@ -80,27 +80,85 @@ let is_elected s ldr =
                   voters in
   is_quorum ldr_voters
 
+(*
+ * Z3 options
+ *)
 #set-options "--query_stats --split_queries always"
 #set-options "--z3rlimit 10000"
 
+(*
+ * The monotonicity of leader election
+ *)
 val mono_ldr: state -> state -> Node.t -> prop
 let mono_ldr s1 s2 ldr = 
   is_elected s1 ldr ==> is_elected s2 ldr
 
+(*
+ * The update precondition for every possible update.
+ * We have just one possible update: Vote.
+ *)
 val update_pre: Node.t -> eff -> state -> bool
 let update_pre n (Vote n1 n2) s =  
     n=n1 && (M.sel s.vote_map n = None)
 
+(*
+ * The first verification condition checks that the 
+ * update precondition is indeed a pre-condition, i.e., 
+ * update is generated only if it is satisfied.
+ *)
 val vc1: s:state -> n:Node.t -> eff:eff ->
   Lemma (requires cast_vote s n = Some eff)
         (ensures update_pre self eff s)
 let vc1 s n eff = ()
 
-val vc2: s1:state -> n1:Node.t -> n2:Node.t -> n3:Node.t 
+(*
+ * VC2 checks that an update applied in any state s1
+ * satisfying the pre-condition will result in state s2
+ * that preserves the monotonicity of leader election.
+ *)
+val vc2: s1:state -> n1:Node.t -> eff:eff 
   -> ldr:Node.t 
-  ->  Lemma (requires update_pre n1 (Vote n2 n3) s1)
+  ->  Lemma (requires update_pre n1 eff s1)
             (ensures 
-              mono_ldr s1 ((handle_vote s1 (Vote n2 n3))._2) ldr)
-let vc2 s1 n1 n2 n3 ldr = ()
+              mono_ldr s1 ((handle_vote s1 eff)._2) ldr)
+let vc2 s1 n1 eff dr = ()
 
-val vc3: s1: 
+(*
+ * VC3 checks that update pre-condition is stable w.r.t 
+ * concurrent effects. In particular, if state s1 satsifes 
+ * the pre-condition of two effects, eff1 and eff2, from 
+ * distinct origins (i.e., they are concurrent), then the 
+ * state s2 resulting from applying eff2 to s1 will continue
+ * satisfying the pre-condition of eff1. In other words, the 
+ * concurrent effect eff2 is not blocking eff1 at a remote replica.
+ * Note that vice-versa is also true due to symmetry.
+ *)
+val vc3: s1:state -> orig1:Node.t -> orig2:Node.t 
+  -> eff1:eff -> eff2:eff
+  -> Lemma (requires    update_pre orig1 eff1 s1
+                     /\ update_pre orig2 eff2 s1
+                     /\ orig1 <> orig2)
+           (ensures update_pre orig1 eff1 (handle_vote s1 eff2)._2) 
+let vc3 s1 orig1 orig2 eff1 eff2 = ()
+
+(*
+ * VC4 is the "CRDT VC": it checks that if effects eff1 and eff2
+ * can be concurrent, i.e., their origins are different and there
+ * exists a state s1 that satisfies both their pre-conditions,
+ * then the order in which the effects are applied shouldn't matter.
+ *)
+val vc4: s1:state -> orig1:Node.t -> orig2:Node.t 
+  -> eff1:eff -> eff2:eff
+  -> Lemma (requires    update_pre orig1 eff1 s1
+                     /\ update_pre orig2 eff2 s1
+                     /\ orig1 <> orig2)
+            (ensures 
+              (let s12 = (handle_vote (handle_vote s1 eff1)._2 eff2)._2 in
+               let s21 = (handle_vote (handle_vote s1 eff2)._2 eff1)._2 in
+               M.equal s12.vote_map s21.vote_map))
+let vc4 s1 orig1 orig2 eff1 eff2 = ()
+
+(* Auxiliary VCs *)
+(* Soundness requires our monotonicity relation (`mono_ldr`) 
+ * to be reflexive and transitive, i.e., it must be a pre-order.
+ * Ideally we have to check these properties too. I am eliding them here.)
